MASSIVE refactor, finished accepts_iff_1mod2_accepts

eNFA_Regex_equivalence.lean
@@ -7,322 +7,268 @@ import Mathlib.Computability.EpsilonNFA
 import Mathlib.Data.Set.Basic
 import Mathlib.Data.Fintype.Basic
 
-open Set
+open Set Classical
+
 
 universe u v
-
-open Classical
 variable {alphabet : Type u} [Fintype alphabet] [DecidableEq alphabet]
 
 set_option linter.unusedSectionVars false
 
+
 namespace εNFA
 
-def to_0mod2_εNFA (A : εNFA alphabet ℕ) : εNFA alphabet ℕ := {
+def to_0mod2 (A : εNFA alphabet ℕ) : εNFA alphabet ℕ := {
     start  := { 2*q' | q' ∈ A.start  }
     accept := { 2*q' | q' ∈ A.accept }
     step   := fun q c =>
         if q % 2 == 0 then
-            {2*q' | q' ∈ (A.step (q/2) c) }
+            { 2*q' | q' ∈ (A.step (q/2) c) }
         else
             ∅
     : εNFA alphabet ℕ
 }
 
-def to_1mod2_εNFA (A : εNFA alphabet ℕ) : εNFA alphabet ℕ := {
+def to_1mod2 (A : εNFA alphabet ℕ) : εNFA alphabet ℕ := {
     start  := { 2*q' + 1 | q' ∈ A.start  }
     accept := { 2*q' + 1 | q' ∈ A.accept }
     step   := fun q c =>
         if q % 2 == 1 then
-            {2*q' + 1 | q' ∈ (A.step ((q - 1)/2) c) }
+            { 2*q' + 1 | q' ∈ (A.step ((q - 1)/2) c) }
         else
             ∅
     : εNFA alphabet ℕ
 }
 
-def is_0mod2_εNFA (A' : εNFA alphabet ℕ) :=
-    ∃ (A : εNFA alphabet ℕ), A' = A.to_0mod2_εNFA
+def is_0mod2 (A' : εNFA alphabet ℕ) :=
+    ∃ (A : εNFA alphabet ℕ), A' = to_0mod2 A
 
-def is_1mod2_εNFA (A' : εNFA alphabet ℕ) :=
-    ∃ (A : εNFA alphabet ℕ), A' = A.to_1mod2_εNFA
+def is_1mod2 (A' : εNFA alphabet ℕ) :=
+    ∃ (A : εNFA alphabet ℕ), A' = to_1mod2 A
+
+lemma if_0mod2_step_is_0mod2 (A' : εNFA alphabet ℕ) (hA': A'.is_0mod2) (q₁ q₂ : ℕ) (σ : Option alphabet) : (q₂ ∈ A'.step q₁ σ) → (q₁ % 2 = 0 ∧  q₂ % 2 = 0) := by
+    intro h_step
+    obtain ⟨A, hA⟩ := hA'
+
+    subst hA
+    simp [to_0mod2] at h_step
+    omega
+
+lemma if_1mod2_step_is_1mod2 (A' : εNFA alphabet ℕ) (hA': A'.is_1mod2) (q₁ q₂ : ℕ) (σ : Option alphabet) : (q₂ ∈ A'.step q₁ σ) → (q₁ % 2 = 1 ∧  q₂ % 2 = 1) := by
+    intro h_step
+    obtain ⟨A, hA⟩ := hA'
+
+    subst hA
+    simp [to_1mod2] at h_step
+    omega
+
+
+lemma if_mod2_step_is_same_mod2 (A' : εNFA alphabet ℕ) (q₁ q₂ : ℕ) (σ : Option alphabet) :
+    A'.is_0mod2 ∨ A'.is_1mod2 → (q₂ ∈ A'.step q₁ σ) → (q₁ % 2 = q₂ % 2) := by
+    intro h_mod2_eNFA h_step
+    cases h_mod2_eNFA
+    case inl h_0mod2 =>
+        have := if_0mod2_step_is_0mod2 A' h_0mod2 q₁ q₂ σ h_step
+        omega
+    case inr h_1mod2 =>
+        have := if_1mod2_step_is_1mod2 A' h_1mod2 q₁ q₂ σ h_step
+        omega
+
+lemma if_0mod2_step_is_same_mod2 (A' : εNFA alphabet ℕ) (hA': A'.is_0mod2) (q₁ q₂ : ℕ) (σ : Option alphabet) :
+    (q₂ ∈ A'.step q₁ σ) → (q₁ % 2 = q₂ % 2) := by
+    apply if_mod2_step_is_same_mod2 A' q₁ q₂ σ
+    left
+    exact hA'
+
+lemma if_1mod2_step_is_same_mod2 (A' : εNFA alphabet ℕ) (hA': A'.is_1mod2) (q₁ q₂ : ℕ) (σ : Option alphabet) :
+    (q₂ ∈ A'.step q₁ σ) → (q₁ % 2 = q₂ % 2) := by
+    apply if_mod2_step_is_same_mod2 A' q₁ q₂ σ
+    right
+    exact hA'
+
+lemma if_mod2_path_is_same_mod2 (A' : εNFA alphabet ℕ) (q₁ q₂ : ℕ) (x : List (Option alphabet)):
+    A'.is_0mod2 ∨ A'.is_1mod2 → (A'.IsPath q₁ q₂ x) → (q₁ % 2 = q₂ % 2) := by
+    intro h_mod2_eNFA h_path
+    induction h_path with
+    | nil _ => rfl
+    | cons t q₁ q₂ c tail h_step h_rest h_induction =>
+        have := if_mod2_step_is_same_mod2 A' q₁ t c h_mod2_eNFA h_step
+        omega
+
+lemma if_0mod2_path_is_same_mod2 (A' : εNFA alphabet ℕ) (hA': A'.is_0mod2) (q₁ q₂ : ℕ) (x : List (Option alphabet)) :
+    (A'.IsPath q₁ q₂ x) → (q₁ % 2 = q₂ % 2) := if_mod2_path_is_same_mod2 A' q₁ q₂ x (Or.inl hA')
+
+lemma if_1mod2_path_is_same_mod2 (A' : εNFA alphabet ℕ) (hA': A'.is_1mod2) (q₁ q₂ : ℕ) (x : List (Option alphabet)) :
+    (A'.IsPath q₁ q₂ x) → (q₁ % 2 = q₂ % 2) := if_mod2_path_is_same_mod2 A' q₁ q₂ x (Or.inr hA')
+
+lemma if_mod2_consequences (A' : εNFA alphabet ℕ) (q : ℕ) :
+    (A'.is_0mod2 → ((q ∈ A'.start → (q % 2 = 0)) ∧ (q ∈ A'.accept → (q % 2 = 0)))) ∧
+    (A'.is_1mod2 → ((q ∈ A'.start → (q % 2 = 1)) ∧ (q ∈ A'.accept → (q % 2 = 1)))) := by
+    constructor <;>
+    intro h_is_mod2
+    <;> constructor <;>
+    intro hq
+    <;> obtain ⟨ A, hA ⟩ := h_is_mod2
+    <;> subst hA
+    <;> simp [to_0mod2, to_1mod2] at hq
+    <;> omega
+
+lemma if_0mod2_qs_is_0mod2 (A' : εNFA alphabet ℕ) (hA': A'.is_0mod2) (q : ℕ) (hq: q ∈ A'.start) :
+    (q % 2 = 0) := ((if_mod2_consequences A' q).left hA').left hq
+
+lemma if_1mod2_qs_is_1mod2 (A' : εNFA alphabet ℕ) (hA': A'.is_1mod2) (q : ℕ) (hq: q ∈ A'.start) :
+    (q % 2 = 1) := ((if_mod2_consequences A' q).right hA').left hq
+
+lemma if_0mod2_qf_is_0mod2 (A' : εNFA alphabet ℕ) (hA': A'.is_0mod2) (q : ℕ) (hq: q ∈ A'.accept) :
+    (q % 2 = 0) := ((if_mod2_consequences A' q).left hA').right hq
+
+lemma if_1mod2_qf_is_1mod2 (A' : εNFA alphabet ℕ) (hA': A'.is_1mod2) (q : ℕ) (hq: q ∈ A'.accept) :
+    (q % 2 = 1) := ((if_mod2_consequences A' q).right hA').right hq
+
+lemma path_iff_mod2_path (A : εNFA alphabet ℕ) (A' : εNFA alphabet ℕ) (qs qf qs' qf' : ℕ) (y : List (Option alphabet)) :
+    (((A' = A.to_0mod2) ∧ (qs' = 2 * qs)     ∧ (qf' = 2 * qf)) ∨
+     ((A' = A.to_1mod2) ∧ (qs' = 2 * qs + 1) ∧ (qf' = 2 * qf + 1))) →
+     ((A.IsPath qs qf y) ↔ (A'.IsPath qs' qf' y)) := by
+
+    rintro (⟨ hA', h_qs', h_qf' ⟩ | ⟨ hA', h_qs', h_qf' ⟩)
+
+    focus
+        let s := 0
+        have h_A'_mod2: A'.is_0mod2 := by use A
+    swap
+    focus
+        let s := 1
+        have h_A'_mod2: A'.is_1mod2 := by use A
+
+    all_goals constructor
+    case inl.mp | inr.mp =>
+        intro h_path_in_A
+        induction h_path_in_A generalizing qs'
+        case nil => simp [εNFA.isPath_nil]; omega
+        case cons t q₁ q₂ σ tail h_step h_path h_induction =>
+            rw [@εNFA.isPath_iff]
+            right
+            let t' := 2 * t + s
+            subst s
+            use t', σ, tail
+            have h_t'_step: t' ∈ A'.step qs' σ := by simp_all [t', to_0mod2, to_1mod2]
+            have h_t'_path: A'.IsPath t' qf' tail := by simp_all [t']
+            exact ⟨ h_t'_step, h_t'_path, rfl ⟩
+
+    case inl.mpr | inr.mpr =>
+        intro h_path_in_A'
+        induction h_path_in_A' generalizing qs
+        case nil => simp [εNFA.isPath_nil]; omega
+        case cons t' q₁' q₂' σ tail h_step h_path h_induction =>
+            rw [@εNFA.isPath_iff]
+            right
+            let t := (t' - s) / 2
+            use t, σ, tail
+
+            have h_t'_0mod2: t' % 2 = s := by
+                try exact (if_0mod2_step_is_0mod2 A' h_A'_mod2 q₁' t' σ h_step).right
+                try exact (if_1mod2_step_is_1mod2 A' h_A'_mod2 q₁' t' σ h_step).right
+            have h_t'_2t: t' = 2 * t + s := by omega
+
+            subst s
+            have h_t_step: t ∈ A.step qs σ := by simp_all [to_0mod2, to_1mod2]
+            have h_t_path: A.IsPath t qf tail := by simp_all
+
+            exact ⟨ h_t_step, h_t_path, rfl ⟩
+
+lemma path_iff_0mod2_path (A : εNFA alphabet ℕ) (A' : εNFA alphabet ℕ) (qs qf qs' qf' : ℕ) (y : List (Option alphabet))
+    (hA': A' = to_0mod2 A) (h_qs': qs' = 2 * qs) (h_qf': qf' = 2 * qf) :
+    (A.IsPath qs qf y) ↔ (A'.IsPath qs' qf' y) :=
+    (path_iff_mod2_path A A' qs qf qs' qf' y (Or.inl ⟨ hA', h_qs', h_qf' ⟩))
+
+lemma path_iff_1mod2_path (A : εNFA alphabet ℕ) (A' : εNFA alphabet ℕ) (qs qf qs' qf' : ℕ) (y : List (Option alphabet))
+    (hA': A' = to_1mod2 A) (h_qs': qs' = 2 * qs + 1) (h_qf': qf' = 2 * qf + 1) :
+    (A.IsPath qs qf y) ↔ (A'.IsPath qs' qf' y) :=
+    (path_iff_mod2_path A A' qs qf qs' qf' y (Or.inr ⟨ hA', h_qs', h_qf' ⟩))
+
+lemma accepts_iff_mod2_accepts (A : εNFA alphabet ℕ) (A' : εNFA alphabet ℕ) :
+    (A' = to_0mod2 A) ∨ (A' = to_1mod2 A) → A.accepts = A'.accepts := by
+    rintro (hA' | hA')
+
+    all_goals
+        rw [@Language.ext_iff]
+        intro x
+        rw [A.mem_accepts_iff_exists_path, A'.mem_accepts_iff_exists_path]
+
+    focus
+        let s := 0
+        have h_A'_mod2: A'.is_0mod2 := by use A
+        have h_A'_start:  A'.start =  { 2*q' + s | q' ∈ A.start  } := by simp_all [s, to_0mod2]
+        have h_A'_accept: A'.accept = { 2*q' + s | q' ∈ A.accept } := by simp_all [s, to_0mod2]
+    swap
+    focus
+        let s := 1
+        have h_A'_mod2: A'.is_1mod2 := by use A
+        have h_A'_start:  A'.start =  { 2*q' + s | q' ∈ A.start  } := by simp_all [s, to_1mod2]
+        have h_A'_accept: A'.accept = { 2*q' + s | q' ∈ A.accept } := by simp_all [s, to_1mod2]
+
+    all_goals constructor
+    case inl.mp | inr.mp =>
+        rintro ⟨ qs, qf, x', h_qs, h_qf, h_x', h_path_in_A ⟩
+        let qs' := 2 * qs + s
+        let qf' := 2 * qf + s
+        subst s
+        have h_qs': qs' ∈ A'.start  := by simp_all [qs']
+        have h_qf': qf' ∈ A'.accept := by simp_all [qf']
+        have h_iff_path : A.IsPath qs qf x' ↔ A'.IsPath qs' qf' x' := by
+            try exact path_iff_mod2_path A A' qs qf qs' qf' x' (Or.inl ⟨ hA', rfl, rfl ⟩)
+            try exact path_iff_mod2_path A A' qs qf qs' qf' x' (Or.inr ⟨ hA', rfl, rfl ⟩)
+
+        use qs', qf', x'
+        exact ⟨ h_qs', h_qf', h_x', h_iff_path.mp h_path_in_A ⟩
+
+    case inl.mpr | inr.mpr =>
+        rintro ⟨ qs', qf', x', h_qs', h_qf', h_x', h_path_in_A' ⟩
+        let qs := (qs' - s) / 2
+        let qf := (qf' - s) / 2
+
+        have h_qs'_qf'_mod2: qs' % 2 = s ∧ qf' % 2 = s := by
+            try exact ⟨ if_0mod2_qs_is_0mod2 A' h_A'_mod2 qs' h_qs', if_0mod2_qf_is_0mod2 A' h_A'_mod2 qf' h_qf' ⟩
+            try exact ⟨ if_1mod2_qs_is_1mod2 A' h_A'_mod2 qs' h_qs', if_1mod2_qf_is_1mod2 A' h_A'_mod2 qf' h_qf' ⟩
+
+        have h_qs'_2qs: qs' = 2 * qs + s := by grind only
+        have h_qf'_2qf: qf' = 2 * qf + s := by grind only
+
+        subst s
+        have h_qs: qs ∈ A.start  := by simp_all
+        have h_qf: qf ∈ A.accept := by simp_all
+        have h_iff_path : A.IsPath qs qf x' ↔ A'.IsPath qs' qf' x' := by
+            try exact path_iff_mod2_path A A' qs qf qs' qf' x' (Or.inl ⟨ hA', h_qs'_2qs, h_qf'_2qf ⟩)
+            try exact path_iff_mod2_path A A' qs qf qs' qf' x' (Or.inr ⟨ hA', h_qs'_2qs, h_qf'_2qf ⟩)
+
+        use qs, qf, x'
+        exact ⟨ h_qs, h_qf, h_x', h_iff_path.mpr h_path_in_A' ⟩
+
+lemma accepts_eq_0mod2_accepts (A : εNFA alphabet ℕ) (A' : εNFA alphabet ℕ) (hA': A' = to_0mod2 A) :
+    A.accepts = A'.accepts := accepts_iff_mod2_accepts A A' (Or.inl hA')
+
+lemma accepts_eq_1mod2_accepts (A : εNFA alphabet ℕ) (A' : εNFA alphabet ℕ) (hA': A' = to_1mod2 A) :
+    A.accepts = A'.accepts := accepts_iff_mod2_accepts A A' (Or.inr hA')
+
+end εNFA
+
+
+namespace εNFA
 
 def contains (A : εNFA alphabet ℕ) (A' : εNFA alphabet ℕ) :=
     ∀ (q : ℕ), ∀ (σ: Option alphabet), A'.step q σ ⊆ A.step q σ
 
-
-lemma reduced_option_append (c : Option alphabet) (tail : List (Option alphabet)) :
-    ([c] ++ tail).reduceOption = [c].reduceOption ++ tail.reduceOption := by
-    exact List.reduceOption_append [c] tail
-
-lemma reduced_option_of_none (c : Option alphabet): c = none → [c].reduceOption = [] := by
-    intro h_c
-    simp [h_c]
-
-lemma path_if_contains (A : εNFA alphabet ℕ) (A' : εNFA alphabet ℕ) :
-    A.contains A' → ∀ (q₁ q₂ : ℕ), ∀ (x : List (Option alphabet)), A'.IsPath q₁ q₂ x → A.IsPath q₁ q₂ x := by
-    intro h_contains q₁ q₂ x h_path
-    unfold εNFA.contains at h_contains
-    induction h_path with
-    | nil q => exact (εNFA.isPath_nil A).mpr rfl
+lemma path_if_contains (A : εNFA alphabet ℕ) (A' : εNFA alphabet ℕ) (h_contains: A.contains A')
+    (q₁ q₂ : ℕ) (x : List (Option alphabet)) :
+    A'.IsPath q₁ q₂ x → A.IsPath q₁ q₂ x := by
+    intro h_path_in_A'
+    unfold contains at h_contains
+    induction h_path_in_A' with
+    | nil q => exact A.isPath_nil.mpr rfl
     | cons t q₁ q₂ c tail h_step h_rest h_induction =>
         constructor
         · exact mem_preimage.mp (h_contains q₁ c h_step)
         · exact h_induction
-
-lemma if_0mod2_step_is_0mod2 (A' : εNFA alphabet ℕ) (hA': A'.is_0mod2_εNFA) (q₁ q₂ : ℕ) (σ : Option alphabet) :
-    (q₂ ∈ A'.step q₁ σ) → (q₁ % 2 = q₂ % 2) := by
-    intro hmem
-    obtain ⟨ A, hA ⟩ := hA'
-    subst hA
-    by_cases h : q₁ % 2 = 0
-    case pos =>
-        have : q₂ ∈ {2*q' | q' ∈ A.step (q₁ / 2) σ} := by
-            simpa [to_0mod2_εNFA, h] using hmem
-        rcases this with ⟨q', _, rfl⟩
-        have h2 : (2 * q') % 2 = 0 :=
-            Nat.mod_eq_zero_of_dvd (dvd_mul_right 2 q')
-        simp [h, h2]
-    case neg =>
-        have : q₂ ∈ (∅ : Set ℕ) := by
-            simp [to_0mod2_εNFA, h] at hmem
-        simp at this
-
-lemma if_1mod2_step_is_1mod2 (A' : εNFA alphabet ℕ) (hA': A'.is_1mod2_εNFA) (q₁ q₂ : ℕ) (σ : Option alphabet) :
-    (q₂ ∈ A'.step q₁ σ) → (q₁ % 2 = q₂ % 2) := by
-    intro hmem
-    obtain ⟨ A, hA ⟩ := hA'
-    subst hA
-    by_cases h : q₁ % 2 = 0
-    case pos =>
-        have : q₂ ∈ (∅ : Set ℕ) := by
-            simp [to_1mod2_εNFA, h] at hmem
-        simp at this
-    case neg =>
-        have : q₂ ∈ {2*q' + 1 | q' ∈ A.step ((q₁ - 1) / 2) σ} := by
-            simp [to_1mod2_εNFA] at hmem
-            obtain ⟨ _, ⟨ q', hmem ⟩ ⟩ := hmem
-            simp only [mem_setOf_eq]
-            use q'
-        rcases this with ⟨q', hq', rfl⟩
-
-        have hodd : q₁ % 2 = 1 := by
-
-            have : q₁ % 2 = 0 ∨ q₁ % 2 = 1 := by
-                exact Nat.mod_two_eq_zero_or_one q₁
-            cases this with
-            | inl hz => exact (h hz).elim
-            | inr ho => exact ho
-
-        have h2 : (2*q' + 1) % 2 = 1 := by
-            simp
-        simp [hodd, h2]
-
-lemma if_0mod2_path_is_0mod2 (A' : εNFA alphabet ℕ) (hA': A'.is_0mod2_εNFA) (q₁ q₂ : ℕ) (x : List (Option alphabet)) :
-    (A'.IsPath q₁ q₂ x) → (q₁ % 2 = q₂ % 2) := by
-    intro hpath
-    have ⟨ A, hA ⟩ := hA'
-    subst hA
-    induction hpath with
-    | nil s =>
-        simp only
-    | cons t s u a x hstep hrest ih =>
-        have hst : s % 2 = t % 2 := by
-            exact if_0mod2_step_is_0mod2 A.to_0mod2_εNFA hA' s t a hstep
-        exact Eq.trans hst ih
-
-
-lemma if_1mod2_path_is_1mod2 (A' : εNFA alphabet ℕ) (hA': A'.is_1mod2_εNFA) (q₁ q₂ : ℕ) (x : List (Option alphabet)) :
-    (A'.IsPath q₁ q₂ x) → (q₁ % 2 = q₂ % 2) := by
-    intro hpath
-    have ⟨ A, hA ⟩ := hA'
-    subst hA
-    induction hpath with
-    | nil s =>
-        simp only
-    | cons t s u a x hstep hrest ih =>
-        have hst : s % 2 = t % 2 := by
-            exact if_1mod2_step_is_1mod2 A.to_1mod2_εNFA hA' s t a hstep
-        exact Eq.trans hst ih
-
-lemma if_0mod2_qs_is_0mod2 (A' : εNFA alphabet ℕ) (hA': A'.is_0mod2_εNFA) (q : ℕ) :
-    q ∈ A'.start → (q % 2 = 0) := by
-    intro hq
-    have ⟨ A, hA ⟩ := hA'
-    subst hA
-    simp [to_0mod2_εNFA] at hq
-    rcases hq with ⟨q', _hq'inStart, rfl⟩
-    exact Nat.mod_eq_zero_of_dvd (dvd_mul_right 2 q')
-
-lemma if_1mod2_qs_is_1mod2 (A' : εNFA alphabet ℕ) (hA': A'.is_1mod2_εNFA)  (q : ℕ) :
-    q ∈ A'.start → (q % 2 = 1) := by
-    intro hq
-    have ⟨ A, hA ⟩ := hA'
-    subst hA
-    simp [to_1mod2_εNFA] at hq
-    rcases hq with ⟨q', _hq'inStart, rfl⟩
-    simp only [Nat.mul_add_mod_self_left, Nat.mod_succ]
-
-lemma if_0mod2_qf_is_0mod2 (A' : εNFA alphabet ℕ) (hA': A'.is_0mod2_εNFA) (q : ℕ) :
-    q ∈ A'.accept → (q % 2 = 0) := by
-    intro hq
-    have ⟨ A, hA ⟩ := hA'
-    subst hA
-    simp [to_0mod2_εNFA] at hq
-    rcases hq with ⟨q', _hq'inStart, rfl⟩
-    exact Nat.mod_eq_zero_of_dvd (dvd_mul_right 2 q')
-
-lemma if_1mod2_qf_is_1mod2 (A' : εNFA alphabet ℕ) (hA': A'.is_1mod2_εNFA)  (q : ℕ) :
-    q ∈ A'.accept → (q % 2 = 1) := by
-    intro hq
-    have ⟨ A, hA ⟩ := hA'
-    subst hA
-    simp [to_1mod2_εNFA] at hq
-    rcases hq with ⟨q', _hq'inStart, rfl⟩
-    simp only [Nat.mul_add_mod_self_left, Nat.mod_succ]
-
-lemma accepts_eq_0mod2_accepts (A : εNFA alphabet ℕ) (A' : εNFA alphabet ℕ) :
-    (A' = to_0mod2_εNFA A) → A.accepts = A'.accepts := by
-    intro hmodzero
-    have hA'start: A'.start = { 2*q' | q' ∈ A.start  } := by
-        rw [hmodzero]
-        unfold to_0mod2_εNFA
-        rw [@setOf_exists]
-    have hA'accept: A'.accept = { 2*q' | q' ∈ A.accept  } := by
-        rw [hmodzero]
-        unfold to_0mod2_εNFA
-        rw [@setOf_exists]
-
-    refine Language.ext_iff.mpr ?_
-    intro x
-    rw [A.mem_accepts_iff_exists_path, A'.mem_accepts_iff_exists_path]
-    constructor
-
-    case mp =>
-        rintro ⟨ q_start, q_accept, x', h_q_start, h_q_accept, h_x', h_ispath ⟩
-        let q'_start := 2 * q_start
-        have h_q'_start: q'_start ∈ A'.start := by
-            simp_all only [q'_start]
-            rw [@mem_setOf_eq]
-            use q_start
-        let q'_accept := 2 * q_accept
-        have h_q'_accept: q'_accept ∈ A'.accept := by
-            simp_all only [q'_accept]
-            rw [@mem_setOf_eq]
-            use q_accept
-
-        use q'_start, q'_accept, x'
-        refine ⟨ h_q'_start, h_q'_accept, h_x' , ?_⟩
-
-        have h_A_path_A'_path: (q₁ q₂ q'₁ q'₂ : ℕ) → (y : List (Option alphabet)) → (q'₁ = 2 * q₁) → (q'₂ = 2* q₂) → (A.IsPath q₁ q₂ y) → (A'.IsPath q'₁ q'₂ y) := by
-            intro q₁ q₂ q'₁ q'₂ y hq'1 hq'2 h_A_path
-            induction h_A_path generalizing q'₁
-            case nil _ _ q_same=>
-                rw [@εNFA.isPath_iff]
-                left
-                rw [hq'1]
-                rw [hq'2]
-                refine ⟨ rfl, rfl ⟩
-            case cons _ _ q_mid q_prev q_final σ tail h_prev_to_mid h_path_mid_to_final h_induction=>
-                rw [@εNFA.isPath_iff]
-                right
-                let q'_mid := 2 * q_mid
-                use q'_mid, σ, tail
-                constructor
-                case left =>
-                    unfold q'_mid
-                    rw [hq'1]
-                    rw [hmodzero]
-                    unfold to_0mod2_εNFA
-                    simp_all
-                case right =>
-                    refine ⟨ ?_, rfl ⟩
-                    unfold q'_mid
-                    rw [hq'2]
-                    rw [hq'2] at h_induction
-                    apply h_induction
-                    rfl
-                    rfl
-
-        apply h_A_path_A'_path q_start q_accept
-        rfl
-        rfl
-        exact h_ispath
-    case mpr =>
-        rintro ⟨ q'_start, q'_accept, x', h_q'_start, h_q'_accept, h_x', h_ispath ⟩
-        let q_start := q'_start / 2
-        have h_q_start: q_start ∈ A.start := by
-            rw [hA'start] at h_q'_start
-            simp at h_q'_start
-            obtain ⟨ q_orig, h_q_orig_tot ⟩ := h_q'_start
-            have horig_is_even: 2 * q_orig = q'_start := by exact h_q_orig_tot.right
-            have h_orig_is_start : q_orig = q_start := by
-                simp [q_start]
-                symm
-                symm at horig_is_even
-                rw [horig_is_even]
-                simp
-            symm at h_orig_is_start
-            rw [h_orig_is_start]
-            exact h_q_orig_tot.left
-        let q_accept := q'_accept / 2
-        have h_q_accept: q_accept ∈ A.accept := by
-            rw [hA'accept] at h_q'_accept
-            simp at h_q'_accept
-            obtain ⟨ q_orig, h_q_orig_tot ⟩ := h_q'_accept
-            have horig_is_even: 2 * q_orig = q'_accept := by exact h_q_orig_tot.right
-            have h_orig_is_accept : q_orig = q_accept := by
-                simp [q_accept]
-                symm
-                symm at horig_is_even
-                rw [horig_is_even]
-                simp
-            symm at h_orig_is_accept
-            rw [h_orig_is_accept]
-            exact h_q_orig_tot.left
-
-        use q_start, q_accept, x'
-        refine ⟨ h_q_start, h_q_accept, h_x' , ?_⟩
-
-        have h_A'_path_A_path: (q₁ q₂ q'₁ q'₂ : ℕ) → (y : List (Option alphabet)) → (q₁ = q'₁ / 2) → (q₂ = q'₂ / 2) → (A'.IsPath q'₁ q'₂ y) → (A.IsPath q₁ q₂ y) := by
-            intro q₁ q₂ q'₁ q'₂ y hq1 hq2 h_A_path
-            induction h_A_path generalizing q₁
-            case nil _ _ q_same=>
-                rw [@εNFA.isPath_iff]
-                left
-                rw [hq1]
-                rw [hq2]
-                refine ⟨ rfl, rfl ⟩
-            case cons _ _ t q₁ q₂ c tail h_step h_path h_induction =>
-                subst hq1 hq2
-                simp at h_induction
-                rw [@εNFA.isPath_iff]
-                right
-                let q_mid := t / 2
-                use q_mid, c, tail
-                constructor
-                case left =>
-                    unfold q_mid
-                    simp only [hmodzero, to_0mod2_εNFA] at h_step
-                    split_ifs at h_step
-                    case pos h_0mod2 =>
-                        obtain ⟨ q', ⟨ hq', ht ⟩ ⟩ := h_step
-                        subst ht
-                        simp
-                        exact mem_of_subset_of_mem (fun ⦃a⦄ a_1 ↦ a_1) hq'
-                    case neg h_1mod2 => simp at h_step
-                case right =>
-                    refine ⟨ ?_, rfl ⟩
-                    unfold q_mid
-                    apply h_induction
-
-        apply h_A'_path_A_path q_start q_accept
-        rfl
-        rfl
-        exact h_ispath
-
-lemma accepts_eq_1mod2_accepts (A : εNFA alphabet ℕ) (A' : εNFA alphabet ℕ) :
-    (A' = to_1mod2_εNFA A) → A.accepts = A'.accepts := by
-    sorry
 
 
  -- -- -- -- -- -- -- -- -- -- --
@@ -338,8 +284,8 @@ def εNFA_zero : εNFA alphabet ℕ := {
 lemma Zero_Regex_to_εNFA :
     ∃ (A: εNFA alphabet ℕ), RegularExpression.zero.matches' = A.accepts := by
         use εNFA_zero
-        simp only [RegularExpression.zero_def, RegularExpression.matches'_zero, Language.zero_def,
-            εNFA.accepts, mem_empty_iff_false, false_and, exists_false, setOf_false, εNFA_zero]
+        simp [εNFA_zero, εNFA.accepts, Language.zero_def]
+
 
  -- -- -- -- -- -- -- -- -- -- -- --
 -- -- -- -- -- EPSILON -- -- -- -- --
@@ -363,7 +309,7 @@ lemma Epsilon_Regex_to_εNFA :
         case mp =>
             intro hx
             use 0, 0, []
-            exact ⟨ rfl, rfl, id (Eq.symm hx), (εNFA.isPath_nil A).mpr rfl ⟩
+            exact ⟨ rfl, rfl, id (Eq.symm hx), (A.isPath_nil).mpr rfl ⟩
 
         case mpr =>
             rintro ⟨ q_start, q_accept, x', h_q_start, h_q_accept, h_x', h_ispath ⟩
@@ -371,6 +317,7 @@ lemma Epsilon_Regex_to_εNFA :
             case nil => exact id (Eq.symm h_x')
             case cons _ _ _ h_step _ =>
                 exact False.elim h_step
+
 
  -- -- -- -- -- -- -- -- -- -- --
 -- -- -- -- -- CHAR -- -- -- -- --
@@ -400,49 +347,42 @@ lemma Char_Regex_to_εNFA (σ : alphabet) :
             intro hx
             use 0, 1, [σ]
             simp
-            refine ⟨ rfl, rfl, ?_, ?_ ⟩
-            · exact id (Eq.symm hx)
-            · simp only [A, εNFA_char, and_self, ↓reduceIte, mem_singleton_iff]
+            have : 1 ∈ A.step 0 (some σ) := by simp [A, εNFA_char]
+            refine ⟨ rfl, rfl, symm hx, this ⟩
 
         case mpr =>
-            rintro ⟨ q_start, q_accept, x', h_q_start, h_q_accept, h_x', h_ispath ⟩
+            rintro ⟨ qs, qf, x', h_qs, h_qf, h_x', h_ispath ⟩
 
             cases h_ispath
-            case nil =>
-                subst h_x'
-                simp_all only [mem_singleton_iff, zero_ne_one, A, εNFA_char]
+            case nil => simp_all [A, εNFA_char]
             case cons t c tail _ h_step =>
                 cases c
                 case none h_none =>
                     absurd h_none
-                    subst A
-                    simp [εNFA_char]
+                    simp [A, εNFA_char]
+
                 case some c h_some =>
-                    by_cases c = σ
-                    case neg h_σ' =>
-                        absurd h_some
-                        subst A
-                        subst h_x'
-                        simp_all only [εNFA_char, mem_singleton_iff, Option.some.injEq, and_false, ↓reduceIte,
-                          mem_empty_iff_false]
-                    case pos h_σ =>
+                    by_cases h_σ: c = σ
+                    case pos =>
                         cases tail
                         case nil =>
-                            subst A
-                            simp only at *
-                            rw[h_σ] at h_x'
-                            exact id (Eq.symm h_x')
+                            subst A h_σ
+                            exact symm h_x'
                         case cons c' _ =>
-                            rw[h_σ] at h_some
-                            unfold A at h_some
+                            subst h_σ A
                             simp [εNFA_char] at h_some
                             rw [h_some.right] at h_step
                             cases h_step
                             case cons t₂ h_t₂ _ =>
                                 absurd h_t₂
-                                subst A
-                                simp only [εNFA_char, one_ne_zero, false_and, ↓reduceIte, mem_empty_iff_false,
-                                  not_false_eq_true]
+                                simp [εNFA_char]
+                    case neg =>
+                        subst h_x' A
+                        absurd h_some
+                        simp [εNFA_char]
+                        intro h_qs h_qc
+                        simp [h_σ] at h_qc -- contradiction
+
 
  -- -- -- -- -- -- -- -- -- -- --
 -- -- -- -- -- PLUS -- -- -- -- --
@@ -466,10 +406,10 @@ lemma Plus_Regex_to_εNFA (r₁ r₂ : RegularExpression alphabet) :
     obtain ⟨ A₁, hA₁ ⟩ := h_r₁
     obtain ⟨ A₂, hA₂ ⟩ := h_r₂
 
-    let A₁' := A₁.to_0mod2_εNFA
-    let A₂' := A₂.to_1mod2_εNFA
-    have hA₁' : A₁'.is_0mod2_εNFA := by use A₁
-    have hA₂' : A₂'.is_1mod2_εNFA := by use A₂
+    let A₁' := A₁.to_0mod2
+    let A₂' := A₂.to_1mod2
+    have hA₁' : A₁'.is_0mod2 := by use A₁
+    have hA₂' : A₂'.is_1mod2 := by use A₂
 
     let A : εNFA alphabet ℕ := εNFA_plus A₁' A₂'
     use A
@@ -479,33 +419,31 @@ lemma Plus_Regex_to_εNFA (r₁ r₂ : RegularExpression alphabet) :
         intro q σ
         by_cases q % 2 = 0
         case pos h_0mod2 => simp [A, εNFA_plus, h_0mod2]
-        case neg h_1mod2 => simp [A₁', to_0mod2_εNFA, h_1mod2]
+        case neg h_1mod2 => simp [A₁', to_0mod2, h_1mod2]
 
     have h_A_contains_A₂' : A.contains A₂' := by
         unfold εNFA.contains
         intro q σ
         by_cases q % 2 = 1
         case pos h_1mod2 => simp [A, εNFA_plus, h_1mod2]
-        case neg h_0mod2 => simp [A₂', to_1mod2_εNFA, h_0mod2]
+        case neg h_0mod2 => simp [A₂', to_1mod2, h_0mod2]
 
     have h_A_path_implies_eq_mod2: (q₁ : ℕ) → (q₂ : ℕ) → (y' : List (Option alphabet)) → (A.IsPath q₁ q₂ y') → (q₁ % 2 = q₂ % 2) := by
         intro q₁ q₂ y' h_is_path
         induction h_is_path
         case nil => exact rfl
         case cons _ _ t q₁ q₂ c y' h_step h_path h_induction =>
-            rw [Eq.symm h_induction]
-            unfold A at h_step
-            simp only at *
+            rw [symm h_induction]
+            simp_rw [A, εNFA_plus] at h_step
             by_cases q₁ % 2 = 0
             case pos h_q₁_0mod2 =>
-                simp_rw [εNFA_plus, h_q₁_0mod2] at h_step
-                exact if_0mod2_step_is_0mod2 A₁' hA₁' q₁ t c h_step
+                simp_rw [h_q₁_0mod2] at h_step
+                exact if_0mod2_step_is_same_mod2 A₁' hA₁' q₁ t c h_step
             case neg h_q₁_1mod2 =>
-                simp_rw [εNFA_plus, h_q₁_1mod2] at h_step
-                exact if_1mod2_step_is_1mod2 A₂' hA₂' q₁ t c h_step
+                simp_rw [h_q₁_1mod2] at h_step
+                exact if_1mod2_step_is_same_mod2 A₂' hA₂' q₁ t c h_step
 
-    simp
-    rw [hA₁, hA₂, @Language.add_def, @Language.ext_iff]
+    simp [hA₁, hA₂, @Language.add_def, @Language.ext_iff]
     intro x
     constructor
     case mp =>
@@ -516,22 +454,20 @@ lemma Plus_Regex_to_εNFA (r₁ r₂ : RegularExpression alphabet) :
             rw [A.mem_accepts_iff_exists_path]
             obtain ⟨ s₁, s₂, x', h_s₁, h_s₂, h_x', h_A₁'_path ⟩ := h_in_A₁
             use s₁, s₂, x'
-            refine ⟨ ?_, ?_, ?_, ?_ ⟩
-            · exact mem_union_left A₂'.start h_s₁
-            · exact mem_union_left A₂'.accept h_s₂
-            · exact h_x'
-            · exact path_if_contains A A₁' h_A_contains_A₁' s₁ s₂ x' h_A₁'_path
+            exact ⟨ mem_union_left A₂'.start h_s₁,
+                    mem_union_left A₂'.accept h_s₂,
+                    h_x',
+                    path_if_contains A A₁' h_A_contains_A₁' s₁ s₂ x' h_A₁'_path ⟩
 
         case inr h_in_A₂ =>
             rw [accepts_eq_1mod2_accepts A₂ A₂' rfl, A₂'.mem_accepts_iff_exists_path] at h_in_A₂
             rw [A.mem_accepts_iff_exists_path]
             obtain ⟨ s₁, s₂, x', h_s₁, h_s₂, h_x', h_A₂'_path ⟩ := h_in_A₂
             use s₁, s₂, x'
-            refine ⟨ ?_, ?_, ?_, ?_ ⟩
-            · exact mem_union_right A₁'.start h_s₁
-            · exact mem_union_right A₁'.accept h_s₂
-            · exact h_x'
-            · exact path_if_contains A A₂' h_A_contains_A₂' s₁ s₂ x' h_A₂'_path
+            exact ⟨ mem_union_right A₁'.start h_s₁,
+                    mem_union_right A₁'.accept h_s₂,
+                    h_x',
+                    path_if_contains A A₂' h_A_contains_A₂' s₁ s₂ x' h_A₂'_path ⟩
 
     case mpr =>
         intro h_in_A
@@ -541,108 +477,111 @@ lemma Plus_Regex_to_εNFA (r₁ r₂ : RegularExpression alphabet) :
         by_cases (qs % 2) = 0
         case pos h_qs_is_0mod2 =>
             left
-            rw [accepts_eq_0mod2_accepts A₁ A₁' rfl]
-            rw [A₁'.mem_accepts_iff_exists_path]
+            rw [accepts_eq_0mod2_accepts A₁ A₁' rfl, A₁'.mem_accepts_iff_exists_path]
             use qs, qf, x'
-            refine ⟨ ?_, ?_, ?_, ?_ ⟩
-            ·   simp [A] at h_qs
+
+            have h_qs_start : qs ∈ A₁'.start := by
+                simp [A] at h_qs
                 cases h_qs
                 case inl h_in_A₁' => exact h_in_A₁'
                 case inr h_in_A₂' =>
                     absurd h_qs_is_0mod2
                     simp
                     exact if_1mod2_qs_is_1mod2 A₂' hA₂' qs h_in_A₂'
-            ·   by_cases (qf % 2) = 0
+
+            have h_qf_accept : qf ∈ A₁'.accept := by
+                by_cases (qf % 2) = 0
                 case pos h_qf_is_0mod2 =>
                     simp [A] at h_qf
                     cases h_qf
                     case inl h_qf_in_A₁'_accept => exact h_qf_in_A₁'_accept
                     case inr h_qf_in_A₂'_accept =>
-                        have : qf % 2 = 1 := by
-                            exact if_1mod2_qf_is_1mod2 A₂' hA₂' qf h_qf_in_A₂'_accept
-                        absurd this
+                        absurd if_1mod2_qf_is_1mod2 A₂' hA₂' qf h_qf_in_A₂'_accept
                         simp [h_qf_is_0mod2]
                 case neg h_qf_is_1mod2 =>
                     simp at h_qf_is_1mod2
                     absurd h_qf_is_1mod2
                     simp
-                    have : qs % 2 = qf % 2 := by exact h_A_path_implies_eq_mod2 qs qf x' h_A_path
+                    have : qs % 2 = qf % 2 := h_A_path_implies_eq_mod2 qs qf x' h_A_path
                     rw [h_qs_is_0mod2] at this
-                    exact id (Eq.symm this)
-            · exact h_x'
-            · have : (q₁ : ℕ) → (q₂ : ℕ) → (y' : List (Option alphabet)) → (q₁ % 2 = 0) → (A.IsPath q₁ q₂ y') → (A₁'.IsPath q₁ q₂ y') := by
-                  intro q₁ q₂ y' h_q₁_0mod2 h_A_path
-                  induction h_A_path
-                  case nil qs => exact (εNFA.isPath_nil A₁').mpr rfl
-                  case cons _ _ t q₁ q₂ c tail h_step h_path h_induction =>
-                      unfold A at h_step
-                      simp only at *
-                      simp_rw [εNFA_plus, h_q₁_0mod2] at h_step
-                      simp at h_step
-                      constructor
-                      · exact h_step
-                      · apply h_induction
-                        have :  q₁ % 2 = t % 2 := by
-                            exact if_0mod2_step_is_0mod2 A₁' hA₁' q₁ t c h_step
-                        rw[h_q₁_0mod2] at this
-                        exact Eq.symm this
-              exact this qs qf x' h_qs_is_0mod2 h_A_path
-        case neg h_qs_is_1mod2 =>
-            simp at h_qs_is_1mod2
+                    exact symm this
+
+            have h_path_qs_to_qf_x' : (q₁ : ℕ) → (q₂ : ℕ) → (y' : List (Option alphabet)) → (q₁ % 2 = 0) → (A.IsPath q₁ q₂ y') → (A₁'.IsPath q₁ q₂ y') := by
+                intro q₁ q₂ y' h_q₁_0mod2 h_A_path
+                induction h_A_path
+                case nil qs => exact (εNFA.isPath_nil A₁').mpr rfl
+                case cons _ _ t q₁ q₂ c tail h_step h_path h_induction =>
+                    unfold A at h_step
+                    simp only at *
+                    simp_rw [εNFA_plus, h_q₁_0mod2] at h_step
+                    simp at h_step
+                    constructor
+                    · exact h_step
+                    · apply h_induction
+                      have : q₁ % 2 = t % 2 := if_0mod2_step_is_same_mod2 A₁' hA₁' q₁ t c h_step
+                      rw [h_q₁_0mod2] at this
+                      exact symm this
+
+            exact ⟨ h_qs_start, h_qf_accept, h_x',
+                    h_path_qs_to_qf_x' qs qf x' h_qs_is_0mod2 h_A_path ⟩
+        case neg h_qs_1mod2 =>
+            simp at h_qs_1mod2
             right
             rw [accepts_eq_1mod2_accepts A₂ A₂' rfl]
             rw [A₂'.mem_accepts_iff_exists_path]
             use qs, qf, x'
-            refine ⟨ ?_, ?_, ?_, ?_ ⟩
-            · simp [A] at h_qs
-              cases h_qs
-              case inl h_in_A₁' =>
-                absurd h_qs_is_1mod2
-                simp
-                exact if_0mod2_qs_is_0mod2 A₁' hA₁' qs h_in_A₁'
-              case inr h_in_A₂' => exact h_in_A₂'
-            · by_cases (qf % 2) = 1
-              case pos h_qf_is_1mod2 =>
-                  simp [A] at h_qf
-                  cases h_qf
-                  case inr h_qf_in_A₂'_accept => exact h_qf_in_A₂'_accept
-                  case inl h_qf_in_A₁'_accept =>
-                      have : qf % 2 = 0 := by
-                          exact if_0mod2_qf_is_0mod2 A₁' hA₁' qf h_qf_in_A₁'_accept
-                      absurd this
-                      simp [h_qf_is_1mod2]
-              case neg h_qf_is_0mod2 =>
-                  simp at h_qf_is_0mod2
-                  absurd h_qf_is_0mod2
-                  simp
-                  have : qs % 2 = qf % 2 := by exact h_A_path_implies_eq_mod2 qs qf x' h_A_path
-                  rw [h_qs_is_1mod2] at this
-                  exact id (Eq.symm this)
-            · exact h_x'
-            · have : (q₁ : ℕ) → (q₂ : ℕ) → (y' : List (Option alphabet)) → (q₁ % 2 = 1) → (A.IsPath q₁ q₂ y') → (A₂'.IsPath q₁ q₂ y') := by
-                  intro q₁ q₂ y' h_q₁_1mod2 h_A_path
-                  induction h_A_path
-                  case nil qs => exact (εNFA.isPath_nil A₂').mpr rfl
-                  case cons _ _ t q₁ q₂ c tail h_step h_path h_induction =>
-                      unfold A at h_step
-                      simp only at *
-                      simp_rw [εNFA_plus, h_q₁_1mod2] at h_step
-                      simp at h_step
-                      constructor
-                      · exact h_step
-                      · apply h_induction
-                        have : t % 2 = q₁ % 2 := by
-                          exact Eq.symm (if_1mod2_step_is_1mod2 A₂' hA₂' q₁ t c h_step)
-                        rw[h_q₁_1mod2] at this
-                        exact this
-              exact this qs qf x' h_qs_is_1mod2 h_A_path
+
+            have h_qs_start : qs ∈ A₂'.start := by
+                simp [A] at h_qs
+                cases h_qs
+                case inl h_in_A₁' =>
+                    absurd h_qs_1mod2
+                    simp
+                    exact if_0mod2_qs_is_0mod2 A₁' hA₁' qs h_in_A₁'
+                case inr h_in_A₂' => exact h_in_A₂'
+
+            have h_qf_accept : qf ∈ A₂'.accept := by
+                by_cases (qf % 2) = 1
+                case pos h_qf_1mod2 =>
+                    simp [A] at h_qf
+                    cases h_qf
+                    case inr h_qf_in_A₂'_accept => exact h_qf_in_A₂'_accept
+                    case inl h_qf_in_A₁'_accept =>
+                        absurd if_0mod2_qf_is_0mod2 A₁' hA₁' qf h_qf_in_A₁'_accept
+                        simp [h_qf_1mod2]
+                case neg h_qf_0mod2 =>
+                    simp at h_qf_0mod2
+                    absurd h_qf_0mod2
+                    simp
+                    have : qs % 2 = qf % 2 := h_A_path_implies_eq_mod2 qs qf x' h_A_path
+                    rw [h_qs_1mod2] at this
+                    exact symm this
+
+            have h_path_qs_to_qf_x': (q₁ : ℕ) → (q₂ : ℕ) → (y' : List (Option alphabet)) → (q₁ % 2 = 1) → (A.IsPath q₁ q₂ y') → (A₂'.IsPath q₁ q₂ y') := by
+                intro q₁ q₂ y' h_q₁_1mod2 h_A_path
+                induction h_A_path
+                case nil qs => exact (εNFA.isPath_nil A₂').mpr rfl
+                case cons _ _ t q₁ q₂ c tail h_step h_path h_induction =>
+                    unfold A at h_step
+                    simp only at *
+                    simp_rw [εNFA_plus, h_q₁_1mod2] at h_step
+                    simp at h_step
+                    constructor
+                    · exact h_step
+                    · apply h_induction
+                      have : q₁ % 2 = t % 2 := if_1mod2_step_is_same_mod2 A₂' hA₂' q₁ t c h_step
+                      rw [h_q₁_1mod2] at this
+                      exact symm this
+
+            exact ⟨ h_qs_start, h_qf_accept, h_x',
+                    h_path_qs_to_qf_x' qs qf x' h_qs_1mod2 h_A_path ⟩
 
 
  -- -- -- -- -- -- -- -- -- -- --
 -- -- -- -- -- COMP -- -- -- -- --
  -- -- -- -- -- -- -- -- -- -- --
 
-def εNFA_comp (A₁: εNFA alphabet ℕ) (A₂: εNFA alphabet ℕ) (hA₁ : A₁.is_0mod2_εNFA) (hA₂ : A₂.is_1mod2_εNFA) : εNFA alphabet ℕ := {
+def εNFA_comp (A₁: εNFA alphabet ℕ) (A₂: εNFA alphabet ℕ) (_ : A₁.is_0mod2) (_ : A₂.is_1mod2) : εNFA alphabet ℕ := {
     start  := A₁.start
     accept := A₂.accept
     step   := fun q c =>
@@ -656,15 +595,15 @@ def εNFA_comp (A₁: εNFA alphabet ℕ) (A₂: εNFA alphabet ℕ) (hA₁ : A�
 }
 
 lemma comp_step_1mod2_to_1mod2 (A A₁' A₂': εNFA alphabet ℕ)
-    (hA₁': A₁'.is_0mod2_εNFA) (hA₂': A₂'.is_1mod2_εNFA) (hA: A = εNFA_comp A₁' A₂' hA₁' hA₂') (q₁ q : ℕ)  :
+    (hA₁': A₁'.is_0mod2) (hA₂': A₂'.is_1mod2) (hA: A = εNFA_comp A₁' A₂' hA₁' hA₂') (q₁ q : ℕ)  :
     ∀ (c : Option alphabet), q₁ % 2 = 1 → (q ∈ A.step q₁ c) → q % 2 = 1 := by
     rintro  c h_q₁_1mod2 h_q
     simp [hA, εNFA_comp, h_q₁_1mod2] at h_q
-    have h_q₁_eq_q_mod2 := if_1mod2_step_is_1mod2 A₂' hA₂' (q₁ := q₁) (q₂ := q) c h_q
+    have h_q₁_eq_q_mod2 := if_1mod2_step_is_same_mod2 A₂' hA₂' (q₁ := q₁) (q₂ := q) c h_q
     simp [symm h_q₁_eq_q_mod2, h_q₁_1mod2]
 
 lemma comp_path_1mod2_to_0mod2_is_empty (A A₁' A₂': εNFA alphabet ℕ)
-    (hA₁': A₁'.is_0mod2_εNFA) (hA₂': A₂'.is_1mod2_εNFA) (hA: A = εNFA_comp A₁' A₂' hA₁' hA₂') (q₁ q₂ : ℕ):
+    (hA₁': A₁'.is_0mod2) (hA₂': A₂'.is_1mod2) (hA: A = εNFA_comp A₁' A₂' hA₁' hA₂') (q₁ q₂ : ℕ):
     ∀ (x' : List (Option alphabet)), q₁ % 2 = 1 ∧ q₂ % 2 = 0 → ¬A.IsPath q₁ q₂ x' := by
     rintro x' ⟨ h_q₁, h_q₂ ⟩ h
     induction h with
@@ -682,19 +621,19 @@ lemma comp_path_1mod2_to_0mod2_is_empty (A A₁' A₂': εNFA alphabet ℕ)
             exact Nat.mod_two_ne_one.mpr h_q₂
 
 lemma comp_path_0mod2 (A A₁' A₂': εNFA alphabet ℕ)
-    (hA₁': A₁'.is_0mod2_εNFA) (hA₂': A₂'.is_1mod2_εNFA) (hA: A = εNFA_comp A₁' A₂' hA₁' hA₂')
+    (hA₁': A₁'.is_0mod2) (hA₂': A₂'.is_1mod2) (hA: A = εNFA_comp A₁' A₂' hA₁' hA₂')
     (q₁ q₂ : ℕ) (x' : List (Option alphabet)) :
     A.IsPath q₁ q₂ x' ∧ q₁ % 2 = 0 ∧ q₂ % 2 = 0 →
     ∀ (t : ℕ), ∀ (a' b' : List (Option alphabet)),
     (a' ++ b' = x') ∧ A.IsPath q₁ t a' ∧ A.IsPath t q₂ b' → t % 2 = 0 := by
     rintro ⟨ h_path_x', h_q₁, h_q₂ ⟩ t a' b' ⟨ h_a'b', h_path_q₁_t, h_path_t_q₂ ⟩
     by_contra! h_t_1mod2
-    have h_t_1mod2 : t % 2 = 1 := by exact Nat.mod_two_ne_zero.mp h_t_1mod2
+    have h_t_1mod2 : t % 2 = 1 := Nat.mod_two_ne_zero.mp h_t_1mod2
     absurd h_path_t_q₂
     exact comp_path_1mod2_to_0mod2_is_empty A A₁' A₂' hA₁' hA₂' hA t q₂ b' ⟨ h_t_1mod2, h_q₂ ⟩
 
 lemma comp_path_0mod2_in_A₁' (A A₁' A₂': εNFA alphabet ℕ)
-    (hA₁': A₁'.is_0mod2_εNFA) (hA₂': A₂'.is_1mod2_εNFA) (hA: A = εNFA_comp A₁' A₂' hA₁' hA₂')
+    (hA₁': A₁'.is_0mod2) (hA₂': A₂'.is_1mod2) (hA: A = εNFA_comp A₁' A₂' hA₁' hA₂')
     (q₁ q₂ : ℕ) (x' : List (Option alphabet)) :
     A.IsPath q₁ q₂ x' ∧ q₁ % 2 = 0 ∧ q₂ % 2 = 0 → (A₁'.IsPath q₁ q₂ x') := by
     rintro ⟨ h_path_in_A, h_q₁, h_q₂ ⟩
@@ -724,19 +663,19 @@ lemma comp_path_0mod2_in_A₁' (A A₁' A₂': εNFA alphabet ℕ)
             exact comp_path_1mod2_to_0mod2_is_empty A A₁' A₂' hA₁' hA₂' hA t q₂ tail ⟨ h_t_1mod2, h_q₂ ⟩
 
 lemma comp_path_1mod2 (A A₁' A₂': εNFA alphabet ℕ)
-    (hA₁': A₁'.is_0mod2_εNFA) (hA₂': A₂'.is_1mod2_εNFA) (hA: A = εNFA_comp A₁' A₂' hA₁' hA₂')
+    (hA₁': A₁'.is_0mod2) (hA₂': A₂'.is_1mod2) (hA: A = εNFA_comp A₁' A₂' hA₁' hA₂')
     (q₁ q₂ : ℕ) (x' : List (Option alphabet)) :
     A.IsPath q₁ q₂ x' ∧ q₁ % 2 = 1 ∧ q₂ % 2 = 1 →
     ∀ (t : ℕ), ∀ (a' b' : List (Option alphabet)),
     (a' ++ b' = x') ∧ A.IsPath q₁ t a' ∧ A.IsPath t q₂ b' → t % 2 = 1 := by
     rintro ⟨ h_path_x', h_q₁, h_q₂ ⟩ t a' b' ⟨ h_a'b', h_path_q₁_t, h_path_t_q₂ ⟩
     by_contra! h_t_0mod2
-    have h_t_0mod2 : t % 2 = 0 := by exact Nat.mod_two_ne_one.mp h_t_0mod2
+    have h_t_0mod2 : t % 2 = 0 := Nat.mod_two_ne_one.mp h_t_0mod2
     absurd h_path_q₁_t
     exact comp_path_1mod2_to_0mod2_is_empty A A₁' A₂' hA₁' hA₂' hA q₁ t a' ⟨ h_q₁, h_t_0mod2 ⟩
 
 lemma comp_path_1mod2_in_A₂' (A A₁' A₂': εNFA alphabet ℕ)
-    (hA₁': A₁'.is_0mod2_εNFA) (hA₂': A₂'.is_1mod2_εNFA) (hA: A = εNFA_comp A₁' A₂' hA₁' hA₂')
+    (hA₁': A₁'.is_0mod2) (hA₂': A₂'.is_1mod2) (hA: A = εNFA_comp A₁' A₂' hA₁' hA₂')
     (q₁ q₂ : ℕ) (x' : List (Option alphabet)) :
     A.IsPath q₁ q₂ x' ∧ q₁ % 2 = 1 ∧ q₂ % 2 = 1 → (A₂'.IsPath q₁ q₂ x') := by
     rintro ⟨ h_path_in_A, h_q₁, h_q₂ ⟩
@@ -755,30 +694,30 @@ lemma comp_path_1mod2_in_A₂' (A A₁' A₂': εNFA alphabet ℕ)
         case neg h_t_0mod2 =>
             simp at h_t_0mod2
             simp [hA, εNFA_comp, h_q₁] at h_step
-            have h_t : q₁ % 2 = t % 2 := by
-                exact if_1mod2_step_is_1mod2 A₂' hA₂' q₁ t c h_step
+            have h_t : q₁ % 2 = t % 2 :=
+                if_1mod2_step_is_same_mod2 A₂' hA₂' q₁ t c h_step
             simp [h_q₁, h_t_0mod2] at h_t
 
 lemma comp_step_change_mod_implies_epsilon (A A₁' A₂': εNFA alphabet ℕ)
-    (hA₁': A₁'.is_0mod2_εNFA) (hA₂': A₂'.is_1mod2_εNFA) (hA: A = εNFA_comp A₁' A₂' hA₁' hA₂')
+    (hA₁': A₁'.is_0mod2) (hA₂': A₂'.is_1mod2) (hA: A = εNFA_comp A₁' A₂' hA₁' hA₂')
     (q₁ q₂ : ℕ) (c : Option alphabet) :
     q₂ ∈ A.step q₁ c ∧ q₁ % 2 = 0 ∧ q₂ % 2 = 1 → c = none := by
     rintro ⟨ h_step, h_q₁, h_q₂ ⟩
     by_contra! h_c_some
     simp [hA, εNFA_comp, h_q₁] at h_step
 
-    by_cases q₁ ∈ A₁'.accept
-    case pos h =>
-        simp [h, h_c_some] at h_step
-        have : q₁ % 2 = q₂ % 2 := if_0mod2_step_is_0mod2 A₁' hA₁' q₁ q₂ c h_step
+    by_cases h_q₁_accept: q₁ ∈ A₁'.accept
+    case pos =>
+        simp [h_q₁_accept, h_c_some] at h_step
+        have : q₁ % 2 = q₂ % 2 := if_0mod2_step_is_same_mod2 A₁' hA₁' q₁ q₂ c h_step
         simp [h_q₁, h_q₂] at this
-    case neg h =>
-        simp [h] at h_step
-        have : q₁ % 2 = q₂ % 2 := if_0mod2_step_is_0mod2 A₁' hA₁' q₁ q₂ c h_step
+    case neg =>
+        simp [h_q₁_accept] at h_step
+        have : q₁ % 2 = q₂ % 2 := if_0mod2_step_is_same_mod2 A₁' hA₁' q₁ q₂ c h_step
         simp [h_q₁, h_q₂] at this
 
 lemma comp_path_decomposition (A A₁' A₂': εNFA alphabet ℕ)
-    (hA₁': A₁'.is_0mod2_εNFA) (hA₂': A₂'.is_1mod2_εNFA) (hA: A = εNFA_comp A₁' A₂' hA₁' hA₂') :
+    (hA₁': A₁'.is_0mod2) (hA₂': A₂'.is_1mod2) (hA: A = εNFA_comp A₁' A₂' hA₁' hA₂') :
     ∀ (qs qf : ℕ), ∀ (y : List alphabet), ∀ (y' : List (Option alphabet)),
     qs % 2 = 0 ∧ qf % 2 = 1 ∧ y = y'.reduceOption ∧ A.IsPath qs qf y' →
     ∃ (qf₁ qs₂ : ℕ), ∃ (a' b' : List (Option alphabet)),
@@ -798,23 +737,13 @@ lemma comp_path_decomposition (A A₁' A₂': εNFA alphabet ℕ)
             use qf₁, qs₂, a', b'
 
             have h_y : (a' ++ ([none] ++ b')).reduceOption = y := by
-                -- TODO: SIMPLIFY THIS DISGUSTING MESS
-                rw [h_y']
                 simp [List.reduceOption_append] at h_tail
-                have : (c :: tail).reduceOption = ([c] ++ tail).reduceOption := by exact List.toList_toArray
-                rw [this, List.reduceOption_append]
-                symm
-                rw[List.reduceOption_append]
+                have : (c :: tail).reduceOption = ([c] ++ tail).reduceOption := List.toList_toArray
+                simp_rw [this] at h_y'
+                subst a' h_y'
+                simp_rw [List.reduceOption_append]
                 simp
-                rw [symm h_tail]
-                have : [c].reduceOption ++ (a''.reduceOption ++ b'.reduceOption) =
-                    ([c].reduceOption ++ a''.reduceOption) ++ b'.reduceOption := by
-                    simp [List.append_assoc]
-                rw [this]
-                have : [c].reduceOption ++ a''.reduceOption = a'.reduceOption := by
-                    subst a'
-                    exact Eq.symm (reduced_option_append c a'')
-                simp [this]
+                exact h_tail
 
             have h_evalfrom_qs_qf₁_a' : qf₁ ∈ A.evalFrom {qs} a'.reduceOption := by
                 subst a'
@@ -834,19 +763,25 @@ lemma comp_path_decomposition (A A₁' A₂': εNFA alphabet ℕ)
 
         case neg h_t_1mod2 =>
             simp at h_t_1mod2
+            use qs, t, [c], tail
+
             have h_c_none : c = none :=
                 comp_step_change_mod_implies_epsilon A A₁' A₂' hA₁' hA₂' hA qs t c ⟨ h_step, h_qs, h_t_1mod2 ⟩
-            use qs, t, [c], tail
-            refine ⟨ h_qs, h_t_1mod2, ?_, ?_, ?_, ?_ ⟩
-            · rw [h_y']; exact List.toList_toArray
-            · subst h_c_none
-              simp [List.reduceOption_nil]
-              tauto
-            · exact A.mem_evalFrom_iff_exists_path.mpr ⟨ tail, rfl, h_path ⟩
-            · rw [h_c_none] at h_step; exact h_step
+            subst h_c_none
+
+            have h_y : ([none] ++ ([none] ++ tail)).reduceOption = y := by simp [h_y']
+
+            have h_qs_eval : qs ∈ A.evalFrom {qs} [none].reduceOption := by
+                simp [List.reduceOption_nil]
+                tauto
+
+            have h_qf_eval : qf ∈ A.evalFrom {t} tail.reduceOption :=
+                A.mem_evalFrom_iff_exists_path.mpr ⟨ tail, rfl, h_path ⟩
+
+            exact ⟨ h_qs, h_t_1mod2, h_y, h_qs_eval, h_qf_eval, h_step ⟩
 
 lemma comp_word_decomposition (A A₁' A₂': εNFA alphabet ℕ)
-    (hA₁': A₁'.is_0mod2_εNFA) (hA₂': A₂'.is_1mod2_εNFA) (hA: A = εNFA_comp A₁' A₂' hA₁' hA₂') (x : List alphabet) :
+    (hA₁': A₁'.is_0mod2) (hA₂': A₂'.is_1mod2) (hA: A = εNFA_comp A₁' A₂' hA₁' hA₂') (x : List alphabet) :
     (x ∈ A.accepts) → ∃ (a b : List alphabet), (x = a ++ b) ∧ (a ∈ A₁'.accepts) ∧ (b ∈ A₂'.accepts) := by
     intro h_x
     have ⟨ qs₁, qf₂, x', h_qs₁, h_qf₂, h_x', h_x'_path  ⟩ := A.mem_accepts_iff_exists_path.mp h_x
@@ -860,7 +795,7 @@ lemma comp_word_decomposition (A A₁' A₂': εNFA alphabet ℕ)
     have h_qf₁_A₁'_accept : qf₁ ∈ A₁'.accept := by
         by_contra!
         simp [hA, εNFA_comp, this, h_qf₁] at h_step
-        simp [if_0mod2_step_is_0mod2 A₁' hA₁' qf₁ qs₂ none h_step] at h_qf₁
+        simp [if_0mod2_step_is_same_mod2 A₁' hA₁' qf₁ qs₂ none h_step] at h_qf₁
         simp [h_qf₁] at h_qs₂
 
     have h_qs₂_A₂'_start : qs₂ ∈ A₂'.start := by
@@ -869,25 +804,32 @@ lemma comp_word_decomposition (A A₁' A₂': εNFA alphabet ℕ)
         case pos h_start => exact h_start
         case neg h_no_start =>
             simp [h_no_start] at h_step
-            simp [if_0mod2_step_is_0mod2 A₁' hA₁' qf₁ qs₂ none h_step, h_qs₂] at h_qf₁
+            simp [if_0mod2_step_is_same_mod2 A₁' hA₁' qf₁ qs₂ none h_step, h_qs₂] at h_qf₁
 
     let a := a'.reduceOption
     let b := b'.reduceOption
     use a, b
-    refine ⟨ ?_, ?_, ?_ ⟩
-    · rw[Eq.symm h_a'b']
-      subst a b
-      exact List.reduceOption_append a' ([none] ++ b')
-    · rw[A₁'.mem_accepts_iff_exists_path]
-      obtain ⟨ w, ⟨ h_w, h_path_qs₁_qf₁ ⟩ ⟩ := A.mem_evalFrom_iff_exists_path.mp h_eval_a'
-      use qs₁, qf₁, w
-      have h_A₁'_path_w := comp_path_0mod2_in_A₁' A A₁' A₂' hA₁' hA₂' hA qs₁ qf₁ w  ⟨ h_path_qs₁_qf₁, h_qs₁_0mod2, h_qf₁ ⟩
-      exact ⟨ h_qs₁, h_qf₁_A₁'_accept, h_w, h_A₁'_path_w ⟩
-    · rw[A₂'.mem_accepts_iff_exists_path]
-      obtain ⟨ w, ⟨ h_w, h_path_qs₂_qf₂ ⟩ ⟩ := A.mem_evalFrom_iff_exists_path.mp h_eval_b'
-      use qs₂, qf₂, w
-      have h_A₂'_path_w := comp_path_1mod2_in_A₂' A A₁' A₂' hA₁' hA₂' hA qs₂ qf₂ w ⟨ h_path_qs₂_qf₂, h_qs₂, h_qf₂_1mod2⟩
-      exact ⟨ h_qs₂_A₂'_start, h_qf₂, h_w, h_A₂'_path_w ⟩
+
+    have h_x_ab : x = a ++ b := by
+        rw [Eq.symm h_a'b']
+        subst a b
+        exact List.reduceOption_append a' ([none] ++ b')
+
+    have h_A₁'_accepts_a : a ∈ A₁'.accepts := by
+        rw [A₁'.mem_accepts_iff_exists_path]
+        obtain ⟨ w, ⟨ h_w, h_path_qs₁_qf₁ ⟩ ⟩ := A.mem_evalFrom_iff_exists_path.mp h_eval_a'
+        use qs₁, qf₁, w
+        have h_A₁'_path_w := comp_path_0mod2_in_A₁' A A₁' A₂' hA₁' hA₂' hA qs₁ qf₁ w  ⟨ h_path_qs₁_qf₁, h_qs₁_0mod2, h_qf₁ ⟩
+        exact ⟨ h_qs₁, h_qf₁_A₁'_accept, h_w, h_A₁'_path_w ⟩
+
+    have h_A₂'_accepts_b : b ∈ A₂'.accepts := by
+        rw [A₂'.mem_accepts_iff_exists_path]
+        obtain ⟨ w, ⟨ h_w, h_path_qs₂_qf₂ ⟩ ⟩ := A.mem_evalFrom_iff_exists_path.mp h_eval_b'
+        use qs₂, qf₂, w
+        have h_A₂'_path_w := comp_path_1mod2_in_A₂' A A₁' A₂' hA₁' hA₂' hA qs₂ qf₂ w ⟨ h_path_qs₂_qf₂, h_qs₂, h_qf₂_1mod2⟩
+        exact ⟨ h_qs₂_A₂'_start, h_qf₂, h_w, h_A₂'_path_w ⟩
+
+    exact ⟨ h_x_ab, h_A₁'_accepts_a, h_A₂'_accepts_b ⟩
 
 lemma Comp_Regex_to_εNFA (r₁ r₂ : RegularExpression alphabet) :
      (∃ (A₁: εNFA alphabet ℕ), r₁.matches' = A₁.accepts) →
@@ -897,11 +839,11 @@ lemma Comp_Regex_to_εNFA (r₁ r₂ : RegularExpression alphabet) :
     obtain ⟨ A₁, hA₁ ⟩ := h_r₁
     obtain ⟨ A₂, hA₂ ⟩ := h_r₂
 
-    let A₁' := to_0mod2_εNFA A₁
-    let A₂' := to_1mod2_εNFA A₂
+    let A₁' := A₁.to_0mod2
+    let A₂' := A₂.to_1mod2
 
-    have hA₁' : A₁'.is_0mod2_εNFA := by use A₁
-    have hA₂' : A₂'.is_1mod2_εNFA := by use A₂
+    have hA₁' : A₁'.is_0mod2 := by use A₁
+    have hA₂' : A₂'.is_1mod2 := by use A₂
 
     let A : εNFA alphabet ℕ := εNFA_comp A₁' A₂' hA₁' hA₂'
     use A
@@ -914,14 +856,14 @@ lemma Comp_Regex_to_εNFA (r₁ r₂ : RegularExpression alphabet) :
             simp [A, εNFA_comp, h_0mod2]
             split_ifs <;>
             simp only [subset_union_left, subset_refl]
-        case neg h_1mod2 => simp [A₁', to_0mod2_εNFA, h_1mod2]
+        case neg h_1mod2 => simp [A₁', to_0mod2, h_1mod2]
 
     have h_A_contains_A₂' : A.contains A₂' := by
         unfold εNFA.contains
         intro q σ
         by_cases q % 2 = 1
         case pos h_1mod2 => simp [A, εNFA_comp, h_1mod2]
-        case neg h_0mod2 => simp [A₂', to_1mod2_εNFA, h_0mod2]
+        case neg h_0mod2 => simp [A₂', to_1mod2, h_0mod2]
 
     simp only [RegularExpression.matches']
     rw [hA₁, hA₂, @Language.mul_def, @Language.ext_iff]
@@ -929,50 +871,57 @@ lemma Comp_Regex_to_εNFA (r₁ r₂ : RegularExpression alphabet) :
     constructor
     case mp =>
         intro h_in_image
-        rw[image2] at h_in_image
+        rw [image2] at h_in_image
         obtain ⟨ x₁, h_x₁, x₂, h_x₂, h_comp ⟩ := h_in_image
         rw [accepts_eq_0mod2_accepts A₁ A₁' rfl, A₁'.mem_accepts_iff_exists_path] at h_x₁
         rw [accepts_eq_1mod2_accepts A₂ A₂' rfl, A₂'.mem_accepts_iff_exists_path] at h_x₂
         obtain ⟨ qs₁, qf₁, x₁', h_qs₁, h_qf₁, h_x₁', h_ispath1 ⟩ := h_x₁
         obtain ⟨ qs₂, qf₂, x₂', h_qs₂, h_qf₂, h_x₂', h_ispath2 ⟩ := h_x₂
         rw [A.mem_accepts_iff_exists_path]
-        use qs₁, qf₂, (x₁' ++ ([none] ++ x₂'))
-        refine ⟨ h_qs₁, h_qf₂, ?_, ?_ ⟩
-        · rw [Eq.symm h_comp]
-          subst h_x₁' h_x₂'
-          exact List.reduceOption_append x₁' ([none] ++ x₂')
-        · rw [isPath_append]
-          use qf₁
-          constructor
-          case left => exact path_if_contains A A₁' h_A_contains_A₁' qs₁ qf₁ x₁' h_ispath1
-          case right =>
-            have h_qf1_even : qf₁ % 2 = 0 :=
-                    if_0mod2_qf_is_0mod2 A₁' hA₁' (q := qf₁) h_qf₁
-            have h_step_mem : qs₂ ∈ A.step qf₁ none := by
-                unfold A
-                simp [εNFA_comp, h_qf1_even, h_qf₁]
-                exact mem_union_right (A₁'.step qf₁ none) h_qs₂
-            have h_epsilon : A.IsPath qf₁ qs₂ [none] := by
-                constructor
-                · exact h_step_mem
-                · exact (εNFA.isPath_nil A).mpr rfl
-            have h_connect : ∃ (t : ℕ), A.IsPath qf₁ t [none] ∧ A.IsPath t qf₂ x₂' := by
-                use qs₂
-                constructor
-                case left => exact h_epsilon
-                case right => exact path_if_contains A A₂' h_A_contains_A₂' qs₂ qf₂ x₂' h_ispath2
-            apply A.isPath_append.mpr h_connect
+
+        let x' :=  (x₁' ++ ([none] ++ x₂'))
+        use qs₁, qf₂, x'
+
+        have h_x' : x'.reduceOption = x := by
+            rw [Eq.symm h_comp]
+            subst h_x₁' h_x₂'
+            exact List.reduceOption_append x₁' ([none] ++ x₂')
+
+        have h_A_path_qs₁_qf₂_x : A.IsPath qs₁ qf₂ x' := by
+            rw [isPath_append]
+            use qf₁
+            constructor
+            case left => exact path_if_contains A A₁' h_A_contains_A₁' qs₁ qf₁ x₁' h_ispath1
+            case right =>
+                have h_qf1_even : qf₁ % 2 = 0 :=
+                        if_0mod2_qf_is_0mod2 A₁' hA₁' (q := qf₁) h_qf₁
+                have h_step_mem : qs₂ ∈ A.step qf₁ none := by
+                    unfold A
+                    simp [εNFA_comp, h_qf1_even, h_qf₁]
+                    exact mem_union_right (A₁'.step qf₁ none) h_qs₂
+                have h_epsilon : A.IsPath qf₁ qs₂ [none] := by
+                    constructor
+                    · exact h_step_mem
+                    · exact (εNFA.isPath_nil A).mpr rfl
+                have h_connect : ∃ (t : ℕ), A.IsPath qf₁ t [none] ∧ A.IsPath t qf₂ x₂' := by
+                    use qs₂
+                    constructor
+                    case left => exact h_epsilon
+                    case right => exact path_if_contains A A₂' h_A_contains_A₂' qs₂ qf₂ x₂' h_ispath2
+                apply A.isPath_append.mpr h_connect
+
+        exact ⟨ h_qs₁, h_qf₂, h_x', h_A_path_qs₁_qf₂_x ⟩
 
     case mpr =>
         intro h_in_A
-        rw[image2]
-        rw [accepts_eq_0mod2_accepts A₁ A₁' rfl, accepts_eq_1mod2_accepts A₂ A₂' rfl]
+        rw [image2, accepts_eq_0mod2_accepts A₁ A₁' rfl, accepts_eq_1mod2_accepts A₂ A₂' rfl]
         obtain ⟨ a, b, h_ab, h_a_accept, h_b_accept ⟩ := comp_word_decomposition A A₁' A₂' hA₁' hA₂' rfl x h_in_A
-        rw [A.mem_accepts_iff_exists_path] at h_in_A
-        obtain ⟨ qs₁, qf₂, x', h_qs₁, h_qf₂, h_x', h_ispath ⟩ := h_in_A
         exact ⟨ a, h_a_accept, b, h_b_accept, Eq.symm h_ab ⟩
 
 
+ -- -- -- -- -- -- -- -- -- -- --
+-- -- -- -- -- STAR -- -- -- -- --
+ -- -- -- -- -- -- -- -- -- -- --
 
 def εNFA_kstar (A: εNFA alphabet ℕ) : εNFA alphabet ℕ := {
     start  := {1}
@@ -986,12 +935,11 @@ def εNFA_kstar (A: εNFA alphabet ℕ) : εNFA alphabet ℕ := {
             A.step q c
 }
 
-
 lemma kstar_append (A A' : εNFA alphabet ℕ) (y y₁ y₂ : List alphabet)
-(hA: A = εNFA_kstar A') (hy: y = y₁ ++ y₂) :
+    (hA: A = εNFA_kstar A') (hy: y = y₁ ++ y₂) :
     (y₁ ∈ A.accepts) ∧ (y₂ ∈ A.accepts) → y ∈ A.accepts := by
     intro ⟨ h_y₁_acc, h_y₂_acc ⟩
-    rw[mem_accepts_iff_exists_path] at h_y₁_acc h_y₂_acc ⊢
+    rw [mem_accepts_iff_exists_path] at h_y₁_acc h_y₂_acc ⊢
     obtain ⟨ qs₁, qf₁, y₁', h_qs₁, h_qf₁, h_y₁', h_y₁_path ⟩ := h_y₁_acc
     obtain ⟨ qs₂, qf₂, y₂', h_qs₂, h_qf₂, h_y₂', h_y₂_path ⟩ := h_y₂_acc
     let y' := y₁' ++ ([none] ++ y₂')
@@ -1002,22 +950,19 @@ lemma kstar_append (A A' : εNFA alphabet ℕ) (y y₁ y₂ : List alphabet)
         exact List.reduceOption_append y₁' ([none] ++ y₂')
 
     have h_connect : A.IsPath qf₁ qs₂ [none] := by
-        simp [εNFA.IsPath]
-        have hqf1 : qf₁ = 1 := by
-            simpa [hA, εNFA_kstar] using h_qf₁
-        have hqs2 : qs₂ = 1 := by
-            simpa [hA, εNFA_kstar] using h_qs₂
+        simp at ⊢
+        have hqf1 : qf₁ = 1 := by simpa [hA, εNFA_kstar] using h_qf₁
+        have hqs2 : qs₂ = 1 := by simpa [hA, εNFA_kstar] using h_qs₂
         subst hqf1; subst hqs2
         simp [hA, εNFA_kstar]
-        by_cases hacc : (1 ∈ A'.accept)
-        · simp [hA, εNFA_kstar, hacc]
-        · simp [hA, εNFA_kstar, hacc]
+        by_cases hacc : (1 ∈ A'.accept) <;>
+        simp [hacc]
 
     have h_full_path : A.IsPath qs₁ qf₂ y' := by
         rw [A.isPath_append]
         use qf₁
         constructor
-        case left => exact h_y₁_path
+        case left  => exact h_y₁_path
         case right => rw [A.isPath_append]; use qs₂
 
     exact ⟨ h_qs₁, h_qf₂, h_y', h_full_path ⟩
@@ -1037,22 +982,26 @@ lemma extract_first_chunk
         sorry
 
 lemma kstar_decompose_path
-    (A A' : εNFA alphabet ℕ) (hA': A'.is_0mod2_εNFA) (hA : A = εNFA_kstar A')
-    (qs qf : ℕ) (x : List (Option alphabet)) :
-    A.IsPath qs qf x → x = [] ∨ ∃ (qs' qf' : ℕ), ∃ a b : List alphabet,
-    (x = a ++ b ∧ A.IsPath qs qs' [] ∧ A'.IsPath qs' qf' a ∧ A.IsPath qf' qf b) := by
-    intro h_x_path_in_A
-    by_cases h_qs_eq_qf: x = []
-    case pos => left; exact h_qs_eq_qf
+    (A A' : εNFA alphabet ℕ) (hA': A'.is_0mod2) (hA : A = εNFA_kstar A')
+    (qs qf : ℕ) (x : List alphabet) (x' : List (Option alphabet))
+    (h_x': x'.reduceOption = x) (h_x_not_empty: x ≠ []) (h_A_path_qs_qf_x': A.IsPath qs qf x') :
+    ∃ (qs' qf' : ℕ) (a b : List alphabet) (a' b' : List (Option alphabet)),
+    (a'.reduceOption = a) ∧ (b'.reduceOption = b) ∧
+    (x = a ++ b) ∧ (qs' ∈ A.εClosure {qs}) ∧ (A'.IsPath qs' qf' a') ∧ (A.IsPath qf' qf b') := by
+
+    by_cases h_qs_1: qs = 1
+    case pos =>
+        sorry
     case neg =>
-        right
-        cases h_x_path_in_A
-        case nil => sorry
-        case cons t qs qf c tail h_step h_rest =>
-            sorry
+        sorry
+    -- cases h_x_path_in_A
+    -- case nil =>
+    --     sorry
+    -- case cons t qs qf c tail h_step h_rest =>
+    --     sorry
 
 lemma kstar_accepts_decomposed_nonempty
-    (A A' : εNFA alphabet ℕ) (hA': A'.is_0mod2_εNFA) (hA : A = εNFA_kstar A') (x : List alphabet) :
+    (A A' : εNFA alphabet ℕ) (hA': A'.is_0mod2) (hA : A = εNFA_kstar A') (x : List alphabet) :
     x ∈ A.accepts → x = [] ∨ ∃ a b : List alphabet, x = a ++ b ∧ a ≠ [] ∧ a ∈ A'.accepts ∧ b ∈ A.accepts := by
     intro h_x_in_A
 
@@ -1072,8 +1021,8 @@ lemma kstar_accepts_decomposed_nonempty
             case pos =>
                 cases c with
                 | none =>
-                    simp[h_tail_empty] at h_x
-                    contradiction
+                    simp [h_tail_empty] at h_x
+                    simp [h_x] at h_x_nil
                 | some σ =>
                     absurd h_step
                     simp [hA, εNFA_kstar]
@@ -1089,8 +1038,8 @@ lemma kstar_accepts_decomposed_nonempty
                         subst h_tail_empty h_x
                         exact Eq.symm (List.append_nil [σ])
 
-                    have h_x_σ : x = [σ] := by
-                        exact Multiset.coe_eq_singleton.mp (congrArg Multiset.ofList h_x_σ_nil)
+                    have h_x_σ : x = [σ] :=
+                        Multiset.coe_eq_singleton.mp (congrArg Multiset.ofList h_x_σ_nil)
 
                     refine ⟨ h_x_σ_nil, List.cons_ne_nil σ [], ?_ ⟩
 
@@ -1123,14 +1072,14 @@ lemma kstar_accepts_decomposed_nonempty
                         apply A'.mem_accepts_iff_exists_path.mpr
                         use t, q₂, x'
                         refine ⟨ ?_, hq₂, hx'.left, hx'.right ⟩
-                        have : some σ ≠ none := by exact Option.some_ne_none σ
+                        have : some σ ≠ none := Option.some_ne_none σ
                         rw [hA, εNFA_kstar] at h_step
-                        simp[this] at h_step
+                        simp [this] at h_step
 
 
 
                     case right =>
-                        rw[mem_accepts_iff_exists_path]
+                        rw [mem_accepts_iff_exists_path]
                         use 1, 1, [none]
 
                         simp [hA, εNFA_kstar, h_1_notin_A']
@@ -1140,8 +1089,8 @@ lemma Star_Regex_to_εNFA (r : RegularExpression alphabet) :
     ∃ (A: εNFA alphabet ℕ), (r.star).matches' = A.accepts := by
     intro h_r
     obtain ⟨ Ar, hAr ⟩ := h_r
-    let A' := Ar.to_0mod2_εNFA
-    have hA' : A'.is_0mod2_εNFA := by use Ar
+    let A' := Ar.to_0mod2
+    have hA' : A'.is_0mod2 := by use Ar
 
     let A : εNFA alphabet ℕ := εNFA_kstar A'
     use A
@@ -1149,15 +1098,15 @@ lemma Star_Regex_to_εNFA (r : RegularExpression alphabet) :
     have h_contains: A.contains A' := by
         unfold εNFA.contains
         intro q σ
-        simp[A, εNFA_kstar]
+        simp [A, εNFA_kstar]
         split_ifs
         case pos => exact subset_insert 1 (A'.step q σ)
         case pos h_1 =>
             obtain ⟨ hq_1, h_σ_none ⟩ := h_1
             subst hq_1 h_σ_none
             have h_empty : A'.step 1 none = ∅ := by
-                simp[A', to_0mod2_εNFA]
-            simp[h_empty]
+                simp [A', to_0mod2]
+            simp [h_empty]
 
         case neg => simp [subset_refl]
 
@@ -1174,52 +1123,102 @@ lemma Star_Regex_to_εNFA (r : RegularExpression alphabet) :
         induction L
         case nil =>
             simp_all only [List.not_mem_nil, IsEmpty.forall_iff, implies_true, List.flatten_nil]
-            rw[mem_accepts_iff_exists_path]
+            rw [mem_accepts_iff_exists_path]
             use 1, 1, []
-            simp[A, εNFA_kstar]
+            simp [A, εNFA_kstar]
         case cons head tail h_induction =>
             simp at h_y
             obtain ⟨ h_head, h_tail ⟩ := h_y
             have h_head_acc : head ∈ A.accepts := by
                 rw [A.mem_accepts_iff_exists_path]
                 rw [A'.mem_accepts_iff_exists_path] at h_head
-                obtain ⟨qs1, qf1, headOpt, h_qs1, h_qf1, h_headOpt, h_path⟩ := h_head
-                refine ⟨1, 1, ([none] ++ headOpt ++ [none]), ?_, ?_, ?_, ?_⟩
-                · simp [A, εNFA_kstar]
-                · simp [A, εNFA_kstar]
-                · simpa [List.reduceOption_append, h_headOpt]
-                ·
-                   have h1_not_acc : (1 : ℕ) ∉ A'.accept := by
-                    simp [A', to_0mod2_εNFA]
-                   have h_step1 : qs1 ∈ A.step 1 none := by
-                     simp [A, εNFA_kstar, h1_not_acc, h_qs1]
-                   have h_eps1 : A.IsPath 1 qs1 [none] :=
-                        A.isPath_singleton.mpr h_step1
-                   have h_mid : A.IsPath qs1 qf1 headOpt :=
-                        path_if_contains A A' h_contains qs1 qf1 headOpt h_path
-                   have h_step2 : (1 : ℕ) ∈ A.step qf1 none := by
-                        simp [A, εNFA_kstar, h_qf1]
-                   have h_eps2 : A.IsPath qf1 1 [none] :=
-                        A.isPath_singleton.mpr h_step2
-                   have h_mid' : A.IsPath qs1 1 (headOpt ++ [none]) :=
-                        A.isPath_append.mpr ⟨qf1, h_mid, h_eps2⟩
-                   have h_1_to_qf1 : A.IsPath 1 qf1 ([none] ++ headOpt) :=
-                         A.isPath_append.mpr ⟨qs1, h_eps1, h_mid⟩
-                   have h_full : A.IsPath 1 1 (([none] ++ headOpt) ++ [none]) :=
-                         A.isPath_append.mpr ⟨qf1, h_1_to_qf1, h_eps2⟩
+                obtain ⟨qs, qf, head', h_qs, h_qf, h_head', h_path⟩ := h_head
 
-                   simpa [List.append_assoc] using h_full
+                let connect_head := ([none] ++ head' ++ [none])
+                use 1, 1, connect_head
+
+                have h_start:  1 ∈ A.start  := by simp [A, εNFA_kstar]
+                have h_accept: 1 ∈ A.accept := by simp [A, εNFA_kstar]
+                have h_head: connect_head.reduceOption = head := by
+                    simp [connect_head, List.reduceOption_append, h_head']
+
+                have h_path_qf_to_1_ε: A.IsPath qf 1 [none] := by
+                    simp [isPath_singleton, A, εNFA_kstar, h_qf]
+
+                have h_path_1_to_qs_ε : A.IsPath 1 qs [none] := by
+                    have : (1 : ℕ) ∉ A'.accept := by simp [A', to_0mod2]
+                    simp [A, εNFA_kstar, this, h_qs, isPath_singleton]
+
+                refine ⟨ h_start, h_accept, h_head, ?_ ⟩
+
+                apply A.isPath_append.mpr; use qf
+                refine ⟨ ?_, h_path_qf_to_1_ε ⟩
+
+                apply A.isPath_append.mpr; use qs
+                refine ⟨ h_path_1_to_qs_ε, ?_ ⟩
+
+                exact path_if_contains A A' h_contains qs qf head' h_path
+
             apply h_induction at h_tail
             exact kstar_append A A' (head :: tail).flatten head tail.flatten rfl rfl ⟨ h_head_acc, h_tail⟩
 
     case mpr =>
-        intro h_in_A
-        have hx :
-            ∃ L : List (List alphabet),
-                x = L.flatten ∧ ∀ y ∈ L, y ∈ A'.accepts :=
-            kstar_word_decomposition (A := A) (A' := A') (hA := rfl) (x := x) h_in_A
-        rcases hx with ⟨L, h_flat, h_all⟩
-        exact ⟨L, h_flat, h_all⟩
+        intro h_x_in_A
+        by_cases h_x_empty: x ≠ []
+        case neg => use []; tauto
+        case pos =>
+            rw [mem_accepts_iff_exists_path] at h_x_in_A
+            obtain ⟨ qs, qf, x', ⟨ h_qs, h_qf, h_x', h_path ⟩ ⟩ := h_x_in_A
+
+
+
+            obtain ⟨ qs', qf', a, b, a', b', ⟨ h_a', h_b', h_x_ab, h_A_path_qs_qs'_nil, h_A'_path_qs'_qf'_a, h_A_path_qf'_qf_b ⟩ ⟩ :=
+                kstar_decompose_path A A' hA' rfl qs qf x x' h_x' h_x_empty h_path
+
+            --subst h_qs h_qf
+            --(x' = a ++ b ∧ A.IsPath qs qs' [] ∧ A'.IsPath qs' qf' a ∧ A.IsPath qf' qf b) := by
+            induction h_A_path_qf'_qf_b with
+            | nil q' =>
+                --simp [A, εNFA_kstar] at h_qs h_qf
+                use [a]
+                simp
+                simp at h_b'
+                simp [h_b'] at h_x_ab
+                refine ⟨ h_x_ab , ?_ ⟩
+
+                have h_qs'_start: qs' ∈ A'.start := by
+                    by_cases qs = 1
+                    case pos h_qs_1 =>
+                        subst h_qs_1
+                    cases h_A_path_qs_qs'_nil with
+                    | base _ h_eq =>
+                        simp at h_eq
+                        --simp [A, εNFA_kstar, symm h_eq] at h_qs
+                        --have : qs' % 2 = 1 := by omega
+                        have : a = x := by
+                            exact List.append_cancel_left (congrArg (HAppend.hAppend x) (id (symm h_x_ab)))
+                        subst this
+
+                        cases h_A'_path_qs'_qf'_a with
+                        | nil =>
+                            simp_all only [ne_eq, List.reduceOption_nil, List.nil_eq, A', A]
+                        | cons t q₁ q₂ c tail h_step h_path =>
+
+                            sorry
+
+                    | step => sorry
+
+                sorry
+
+            | cons =>
+                sorry
+
+            have hx :
+                ∃ L : List (List alphabet),
+                    x = L.flatten ∧ ∀ y ∈ L, y ∈ A'.accepts :=
+                    kstar_decompose_path (A := A) (A' := A') (hA := rfl) (x := x) h_in_A
+            rcases hx with ⟨L, h_flat, h_all⟩
+            exact ⟨L, h_flat, h_all⟩
 
 
 
